Makefile
@@ -112,7 +112,7 @@ VFILES:=theories/Tactic.v\
   theories/Tower.v\
   theories/Sequent.v\
   theories/InternalRules.v\
-  theories/FormalTerm.v\
+  theories/ExternalSyn.v\
   theories/ExternalRules.v
 
 ifneq ($(filter-out archclean clean cleanall printenv,$(MAKECMDGOALS)),)
